src/tls/Test.TLS.Send.fst
@@ -1,0 +1,123 @@
+module Test.TLS.Send
+
+module HS = FStar.HyperStack
+module Nego = Negotiation
+module HST = FStar.HyperStack.ST
+module TS = TLS.Handshake.Send
+module T = HSL.Transcript
+module B = LowStar.Buffer
+
+module HSM = Parsers.Handshake
+module HSM12 = Parsers.Handshake12
+module HSM13 = Parsers.Handshake13
+
+
+open FStar.Integers
+open FStar.HyperStack.ST
+open CipherSuite
+open TLSError
+
+// TODO may require switching from Tot to Stack
+assume val trace: string -> unit
+
+noeq type handshake = | HS:
+  #region: Mem.rgn {Mem.is_hs_rgn region} ->
+  r: TLSConstants.role ->
+  nego: Nego.t region r ->
+  #a: EverCrypt.Hash.alg ->
+  stt: TS.transcript_state a ->
+  #n: Ghost.erased nat ->                 // Length of the current transcript
+  t:T.g_transcript_n n ->                // Ghost transcript
+  sto:TS.send_state ->
+//  log: HandshakeLog.t {HandshakeLog.region_of log = region} ->
+//  ks: KeySchedule.ks (*region*) ->
+//  epochs: epochs region (Nego.nonce nego) ->
+//  state: ref machineState {HS.frameOf state = region} -> // state machine; should be opaque and depend on r.
+  handshake
+
+let valid (hs:handshake) (h:HS.mem) =
+  TS.invariant hs.sto h /\
+  T.invariant hs.stt (Ghost.reveal hs.t) h /\
+  h `HS.contains` hs.nego.Nego.state /\
+  B.loc_disjoint (TS.footprint hs.sto) (T.footprint hs.stt) /\
+  B.loc_disjoint (TS.footprint hs.sto) (B.loc_mreference hs.nego.Nego.state) /\
+  B.loc_disjoint (T.footprint hs.stt) (B.loc_mreference hs.nego.Nego.state)
+
+let footprint (hs:handshake) =
+  TS.footprint hs.sto `B.loc_union`
+  T.footprint hs.stt `B.loc_union` 
+  B.loc_mreference hs.nego.Nego.state
+
+let is_state13 (hs:handshake) = T.Transcript13? (Ghost.reveal hs.t)
+
+// TODO: Should be computed using key schedule
+assume val svd:HSM13.handshake13_m13_finished
+//TODO: Should be computed from nego + certificate13 parsers
+assume val cert:HSM13.handshake13_m13_certificate
+// TODO: Should be computed from nego. Requires lowering to take hash instead of bytes?
+assume val signature:HSM13.handshake13_m13_certificate_verify
+
+val serverFinished: hs:handshake -> tag:Hacl.Hash.Definitions.hash_t (hs.a) -> ST (result handshake)
+    (requires fun h -> valid hs h /\ B.live h tag /\ is_state13 hs /\
+      Ghost.reveal hs.n < T.max_transcript_size - 4 /\
+      B.loc_disjoint (B.loc_buffer tag) (B.loc_region_only true Mem.tls_tables_region) /\
+      B.loc_disjoint (B.loc_buffer tag) (footprint hs))
+    (ensures fun h0 res h1 -> 
+      B.(modifies (footprint hs `loc_union` loc_buffer tag `loc_union` loc_region_only true Mem.tls_tables_region)) h0 h1 /\
+      begin match res with
+      | Correct hs' -> valid hs' h1
+      | _ -> True
+      end
+    )
+
+#set-options "--z3rlimit 50"
+
+let serverFinished hs tag =
+    trace "prepare Server Finished";
+    let mode = Nego.getMode hs.nego in
+    let cfg = Nego.local_config hs.nego in
+    let kex = Nego.kexAlg mode in
+    let pv = mode.Nego.n_protocol_version in
+    let cs = mode.Nego.n_cipher_suite in
+    let exts = mode.Nego.n_server_extensions in
+    let eexts = match mode.Nego.n_encrypted_extensions with | None -> [] | Some ee -> ee in
+
+    let digestFinished : result handshake =
+      match kex with
+      | Kex_ECDHE -> // [Certificate; CertificateVerify]
+        let m = HSM13.M13_encrypted_extensions eexts in
+        begin
+        match TS.send13 hs.stt hs.t hs.sto m with
+        | Correct (sto, t') ->
+          let m = HSM13.M13_certificate cert in
+          begin
+          match TS.send_tag13 hs.stt t' sto m tag with
+          | Correct (sto, t') ->
+            begin
+            match TS.send_tag13 hs.stt t' sto (HSM13.M13_certificate_verify signature) tag with
+            | Correct (sto, t') -> Correct (HS hs.r hs.nego hs.stt t' sto)
+            | Error z -> Error z
+            end
+          | Error z -> Error z
+          end
+        | Error z -> Error z
+        end
+      | _ -> // PSK
+        let m = HSM13.M13_encrypted_extensions eexts in
+        match TS.send_tag13 hs.stt hs.t hs.sto m tag with
+        | Correct (sto, t') -> 
+          let h1 = get() in
+          Correct (HS hs.r hs.nego hs.stt t' sto)
+        | Error z -> Error z
+    in
+    match digestFinished with
+    | Correct hs' ->
+      let m = HSM13.M13_finished svd in
+      begin
+      match TS.send_tag13 hs'.stt hs'.t hs'.sto m tag with
+      | Correct (sto, t') ->
+        // TODO: export, register, send signals, nego state
+        Correct (HS hs.r hs.nego hs.stt t' sto)
+      | Error z -> Error z
+      end
+    | Error z -> Error z
